src/Math/NatArith.dfy
@@ -7,5 +7,21 @@ module NatArith {
     if a < b then a else b
   }
 
+  // Computes the rising factorial start^(n),
+  // i.e. the product `start * (start + 1) * ... * (start + n - 1)`, i.e. with n factors.
+  // see: https://en.wikipedia.org/wiki/Falling_and_rising_factorials
+  // With the default value of start = 1, it computes n!
+  // The start parameter is useful for inductive proofs.
+  opaque function Factorial(n: nat, start: nat := 1): nat {
+    if n == 0 then 1 else start * Factorial(n - 1, start + 1)
+  }
+
+  lemma FactoralPositive(n: nat, start: nat := 1)
+    requires start >= 1
+    ensures Factorial(n, start) >= 1
+  {
+    reveal Factorial();
+  }
+
   // TODO: a lot of functions from the helper module should go here.
 }
